Fix extraction. Still problems with the examples

io/case-study/Compiler_MIO_To_Interm.ml
@@ -1,0 +1,2163 @@
+open Prims
+let (get_trace : unit -> unit -> (unit, unit, unit, Obj.t) MIO.dm_gmio) =
+  fun mst ->
+    fun uu___ ->
+      MIO_Sig_Call.mio_call () Free.Prog MIO_Sig.GetTrace (Obj.repr ())
+let (get_state : unit -> unit -> (unit, unit, unit, unit) MIO.dm_gmio) =
+  fun mst ->
+    fun uu___ ->
+      MIO_Sig_Call.mio_call () Free.Prog MIO_Sig.GetST (Obj.repr ())
+type 'a tree =
+  | Leaf 
+  | EmptyNode of 'a tree * 'a tree 
+  | Node of 'a * 'a tree * 'a tree 
+let uu___is_Leaf : 'a . 'a tree -> Prims.bool =
+  fun projectee -> match projectee with | Leaf -> true | uu___ -> false
+let uu___is_EmptyNode : 'a . 'a tree -> Prims.bool =
+  fun projectee ->
+    match projectee with | EmptyNode (left, right) -> true | uu___ -> false
+let __proj__EmptyNode__item__left : 'a . 'a tree -> 'a tree =
+  fun projectee -> match projectee with | EmptyNode (left, right) -> left
+let __proj__EmptyNode__item__right : 'a . 'a tree -> 'a tree =
+  fun projectee -> match projectee with | EmptyNode (left, right) -> right
+let uu___is_Node : 'a . 'a tree -> Prims.bool =
+  fun projectee ->
+    match projectee with | Node (data, left, right) -> true | uu___ -> false
+let __proj__Node__item__data : 'a . 'a tree -> 'a =
+  fun projectee -> match projectee with | Node (data, left, right) -> data
+let __proj__Node__item__left : 'a . 'a tree -> 'a tree =
+  fun projectee -> match projectee with | Node (data, left, right) -> left
+let __proj__Node__item__right : 'a . 'a tree -> 'a tree =
+  fun projectee -> match projectee with | Node (data, left, right) -> right
+let root : 'a . 'a tree -> 'a = fun t -> __proj__Node__item__data t
+let left : 'a . 'a tree -> 'a tree =
+  fun t ->
+    match t with
+    | Node (uu___, lt, uu___1) -> lt
+    | EmptyNode (lt, uu___) -> lt
+let right : 'a . 'a tree -> 'a tree =
+  fun t ->
+    match t with
+    | Node (uu___, uu___1, rt) -> rt
+    | EmptyNode (uu___, rt) -> rt
+type ('a, 't1, 't2) equal_trees = Obj.t
+let rec map_tree : 'a 'b . 'a tree -> ('a -> 'b) -> 'b tree =
+  fun t ->
+    fun f ->
+      match t with
+      | Leaf -> Leaf
+      | EmptyNode (lhs, rhs) ->
+          EmptyNode ((map_tree lhs f), (map_tree rhs f))
+      | Node (x, lhs, rhs) ->
+          Node ((f x), (map_tree lhs f), (map_tree rhs f))
+let (get_local_trace : MIO_Sig.trace -> MIO_Sig.trace -> MIO_Sig.trace) =
+  fun h' ->
+    fun h ->
+      let n =
+        (FStar_List_Tot_Base.length h) - (FStar_List_Tot_Base.length h') in
+      let uu___ = FStar_List_Tot_Base.splitAt n h in
+      match uu___ with | (lt', ht) -> FStar_List_Tot_Base.rev lt'
+type ('argt, 'rett) idc_typ =
+  'argt -> MIO_Sig.trace -> 'rett -> MIO_Sig.trace -> Prims.bool
+type ('mst, 'argt, 'rett) dc_typ_0 =
+  'argt -> Obj.t -> 'rett -> Obj.t -> Prims.bool
+type ('mst, 'argt, 'rett, 'idc) dc_typ = (unit, 'argt, 'rett) dc_typ_0
+type ('a, 'b, 'mst, 'idc, 'dc, 'h0, 'x, 'y, 'h1, 'b1,
+  'lt) eff_dc_typ_cont_post = unit
+type ('mst, 'fl, 't1, 't2, 'idc, 'dc, 'x, 'h0) eff_dc_typ_cont =
+  't2 -> (Prims.bool, unit, unit, unit) MIO.dm_gmio
+type ('mst, 'fl, 't1, 't2, 'idc, 'dc) eff_dc_typ =
+  't1 ->
+    ((unit, unit,
+       (unit, unit, 't1, 't2, unit, unit, unit, unit) eff_dc_typ_cont)
+       FStar_Pervasives.dtuple3,
+      unit, unit, unit) MIO.dm_gmio
+let (enforce_dc :
+  unit ->
+    unit ->
+      unit ->
+        (Obj.t, Obj.t) idc_typ ->
+          (unit, Obj.t, Obj.t, unit) dc_typ ->
+            (unit, unit, Obj.t, Obj.t, unit, unit) eff_dc_typ)
+  =
+  fun uu___4 ->
+    fun uu___3 ->
+      fun uu___2 ->
+        fun uu___1 ->
+          fun uu___ ->
+            (fun mst ->
+               fun argt ->
+                 fun rett ->
+                   fun idc ->
+                     fun dc ->
+                       Obj.magic
+                         (fun x ->
+                            MIO.dm_gmio_bind () () () () () (get_trace () ())
+                              (fun h0 ->
+                                 MIO.dm_gmio_bind () () () () ()
+                                   (Obj.magic (get_state () ()))
+                                   (fun s0 ->
+                                      MIO.lift_pure_dm_gmio () ()
+                                        (fun uu___ ->
+                                           (fun uu___ ->
+                                              Obj.magic
+                                                (FStar_Pervasives.Mkdtuple3
+                                                   (s0, (),
+                                                     (Obj.magic
+                                                        (fun y ->
+                                                           MIO.dm_gmio_bind
+                                                             () () () () ()
+                                                             (get_trace () ())
+                                                             (fun h1 ->
+                                                                MIO.dm_gmio_bind
+                                                                  () () () ()
+                                                                  ()
+                                                                  (Obj.magic
+                                                                    (get_state
+                                                                    () ()))
+                                                                  (fun s1 ->
+                                                                    MIO.lift_pure_dm_gmio
+                                                                    () ()
+                                                                    (fun
+                                                                    uu___1 ->
+                                                                    dc x s0 y
+                                                                    s1))))))))
+                                             uu___))))) uu___4 uu___3 uu___2
+              uu___1 uu___
+type 'mst pck_dc =
+  (unit, unit, (Obj.t, Obj.t) idc_typ, (unit, Obj.t, Obj.t, unit) dc_typ)
+    FStar_Pervasives.dtuple4
+type ('mst, 'ctr) arg_typ = Obj.t
+type ('mst, 'ctr) ret_typ = Obj.t
+type ('mst, 'ctr, 'arg, 'h, 'ret, 'lt) icheck = unit
+let (check :
+  unit -> unit pck_dc -> Obj.t -> Obj.t -> Obj.t -> Obj.t -> Prims.bool) =
+  fun mst ->
+    fun ctr ->
+      fun arg ->
+        fun s0 ->
+          fun ret ->
+            fun s1 ->
+              FStar_Pervasives.__proj__Mkdtuple4__item___4 ctr arg s0 ret s1
+type ('mst, 'fl) eff_pck_dc =
+  (unit pck_dc, (unit, unit, unit, unit, unit, unit) eff_dc_typ)
+    Prims.dtuple2
+let (make_dc_eff : unit -> unit pck_dc -> (unit, unit) eff_pck_dc) =
+  fun mst ->
+    fun r ->
+      Prims.Mkdtuple2
+        (r,
+          (Obj.magic
+             (enforce_dc () () ()
+                (FStar_Pervasives.__proj__Mkdtuple4__item___3 r)
+                (FStar_Pervasives.__proj__Mkdtuple4__item___4 r))))
+type ('mst, 'fl, 'dcs) typ_eff_dcs = (unit, unit) eff_pck_dc tree
+let (typ_left :
+  unit ->
+    unit ->
+      unit pck_dc tree ->
+        (unit, unit, unit) typ_eff_dcs -> (unit, unit, unit) typ_eff_dcs)
+  = fun mst -> fun fl -> fun dcs -> fun t -> left t
+let (typ_right :
+  unit ->
+    unit ->
+      unit pck_dc tree ->
+        (unit, unit, unit) typ_eff_dcs -> (unit, unit, unit) typ_eff_dcs)
+  = fun mst -> fun fl -> fun dcs -> fun t -> right t
+let (make_dcs_eff :
+  unit -> unit pck_dc tree -> (unit, unit, unit) typ_eff_dcs) =
+  fun mst ->
+    fun dcs ->
+      let r = map_tree dcs (make_dc_eff ()) in
+      let comp x = FStar_Pervasives.dfst (make_dc_eff () x) in r
+type ('styp, 'fl, 'pi, 'mst, 'dcs) exportable =
+  {
+  ityp: unit ;
+  c_ityp: (Obj.t, unit, 'pi, unit) Compiler_Languages.interm ;
+  export: (unit, unit, unit) typ_eff_dcs -> 'styp -> Obj.t }
+let __proj__Mkexportable__item__c_ityp :
+  'styp .
+    unit ->
+      unit ->
+        unit ->
+          unit pck_dc tree ->
+            ('styp, unit, Obj.t, unit, unit) exportable ->
+              (unit, unit, Obj.t, unit) Compiler_Languages.interm
+  =
+  fun uu___4 ->
+    fun uu___3 ->
+      fun uu___2 ->
+        fun uu___1 ->
+          fun uu___ ->
+            (fun fl ->
+               fun pi ->
+                 fun mst ->
+                   fun dcs ->
+                     fun projectee ->
+                       match projectee with
+                       | { ityp; c_ityp; export;_} -> Obj.magic c_ityp)
+              uu___4 uu___3 uu___2 uu___1 uu___
+let __proj__Mkexportable__item__export :
+  'styp .
+    unit ->
+      unit ->
+        unit ->
+          unit pck_dc tree ->
+            ('styp, unit, Obj.t, unit, unit) exportable ->
+              (unit, unit, unit) typ_eff_dcs -> 'styp -> Obj.t
+  =
+  fun fl ->
+    fun pi ->
+      fun mst ->
+        fun dcs ->
+          fun projectee ->
+            match projectee with | { ityp; c_ityp; export;_} -> export
+type ('styp, 'fl, 'pi, 'mst, 'dcs) safe_importable =
+  {
+  ityp1: unit ;
+  c_ityp1: (Obj.t, unit, 'pi, unit) Compiler_Languages.interm ;
+  safe_import: Obj.t -> (unit, unit, unit) typ_eff_dcs -> 'styp }
+let __proj__Mksafe_importable__item__c_ityp :
+  'styp .
+    unit ->
+      unit ->
+        unit ->
+          unit pck_dc tree ->
+            ('styp, unit, Obj.t, unit, unit) safe_importable ->
+              (unit, unit, Obj.t, unit) Compiler_Languages.interm
+  =
+  fun uu___4 ->
+    fun uu___3 ->
+      fun uu___2 ->
+        fun uu___1 ->
+          fun uu___ ->
+            (fun fl ->
+               fun pi ->
+                 fun mst ->
+                   fun dcs ->
+                     fun projectee ->
+                       match projectee with
+                       | { ityp1 = ityp; c_ityp1 = c_ityp; safe_import;_} ->
+                           Obj.magic c_ityp) uu___4 uu___3 uu___2 uu___1
+              uu___
+let __proj__Mksafe_importable__item__safe_import :
+  'styp .
+    unit ->
+      unit ->
+        unit ->
+          unit pck_dc tree ->
+            ('styp, unit, Obj.t, unit, unit) safe_importable ->
+              Obj.t -> (unit, unit, unit) typ_eff_dcs -> 'styp
+  =
+  fun fl ->
+    fun pi ->
+      fun mst ->
+        fun dcs ->
+          fun projectee ->
+            match projectee with
+            | { ityp1 = ityp; c_ityp1 = c_ityp; safe_import;_} -> safe_import
+type ('styp, 'fl, 'pi, 'mst, 'dcs) importable =
+  {
+  ityp2: unit ;
+  c_ityp2: (Obj.t, unit, 'pi, unit) Compiler_Languages.interm ;
+  import: Obj.t -> (unit, unit, unit) typ_eff_dcs -> 'styp CommonUtils.resexn }
+let __proj__Mkimportable__item__c_ityp :
+  'styp .
+    unit ->
+      unit ->
+        unit ->
+          unit pck_dc tree ->
+            ('styp, unit, Obj.t, unit, unit) importable ->
+              (unit, unit, Obj.t, unit) Compiler_Languages.interm
+  =
+  fun uu___4 ->
+    fun uu___3 ->
+      fun uu___2 ->
+        fun uu___1 ->
+          fun uu___ ->
+            (fun fl ->
+               fun pi ->
+                 fun mst ->
+                   fun dcs ->
+                     fun projectee ->
+                       match projectee with
+                       | { ityp2 = ityp; c_ityp2 = c_ityp; import;_} ->
+                           Obj.magic c_ityp) uu___4 uu___3 uu___2 uu___1
+              uu___
+let __proj__Mkimportable__item__import :
+  'styp .
+    unit ->
+      unit ->
+        unit ->
+          unit pck_dc tree ->
+            ('styp, unit, Obj.t, unit, unit) importable ->
+              Obj.t ->
+                (unit, unit, unit) typ_eff_dcs -> 'styp CommonUtils.resexn
+  =
+  fun fl ->
+    fun pi ->
+      fun mst ->
+        fun dcs ->
+          fun projectee ->
+            match projectee with
+            | { ityp2 = ityp; c_ityp2 = c_ityp; import;_} -> import
+let interm_importable_super :
+  'styp .
+    unit ->
+      unit ->
+        unit ->
+          unit pck_dc tree ->
+            ('styp, unit, Obj.t, unit, unit) importable ->
+              (unit, unit, Obj.t, unit) Compiler_Languages.interm
+  = fun fl -> fun pi -> fun mst -> fun dcs -> fun d -> Obj.magic d.c_ityp2
+let interm_exportable_super :
+  'styp .
+    unit ->
+      unit ->
+        unit ->
+          unit pck_dc tree ->
+            ('styp, unit, Obj.t, unit, unit) exportable ->
+              (unit, unit, Obj.t, unit) Compiler_Languages.interm
+  = fun fl -> fun pi -> fun mst -> fun dcs -> fun d -> Obj.magic d.c_ityp
+let interm_safe_importable_super :
+  'styp .
+    unit ->
+      unit ->
+        unit ->
+          unit pck_dc tree ->
+            ('styp, unit, Obj.t, unit, unit) safe_importable ->
+              (unit, unit, Obj.t, unit) Compiler_Languages.interm
+  = fun fl -> fun pi -> fun mst -> fun dcs -> fun d -> Obj.magic d.c_ityp1
+let (interm_is_exportable :
+  unit ->
+    unit ->
+      unit ->
+        unit pck_dc tree ->
+          unit ->
+            (Obj.t, unit, Obj.t, unit) Compiler_Languages.interm ->
+              (Obj.t, unit, Obj.t, unit, unit) exportable)
+  =
+  fun fl ->
+    fun pi ->
+      fun mst ->
+        fun dcs ->
+          fun t ->
+            fun d1 ->
+              {
+                ityp = ();
+                c_ityp = d1;
+                export = (fun uu___ -> fun x -> match uu___ with | Leaf -> x)
+              }
+let (exportable_unit :
+  unit -> unit -> unit -> (unit, unit, Obj.t, unit, unit) exportable) =
+  fun fl ->
+    fun pi ->
+      fun mst ->
+        {
+          ityp = ();
+          c_ityp = (Obj.magic (Compiler_Languages.interm_unit () () ()));
+          export =
+            (fun uu___1 ->
+               fun uu___ ->
+                 (fun uu___ -> fun uu___1 -> Obj.magic ()) uu___1 uu___)
+        }
+let (exportable_file_descr :
+  unit ->
+    unit ->
+      unit -> (UnixTypes.file_descr, unit, Obj.t, unit, unit) exportable)
+  =
+  fun fl ->
+    fun pi ->
+      fun mst ->
+        {
+          ityp = ();
+          c_ityp = (Obj.magic (Compiler_Languages.interm_int () () ()));
+          export =
+            (fun uu___1 ->
+               fun uu___ ->
+                 (fun uu___ ->
+                    fun fd -> match uu___ with | Leaf -> Obj.magic fd) uu___1
+                   uu___)
+        }
+let (exportable_bytes :
+  unit ->
+    unit -> unit -> (FStar_Bytes.bytes, unit, Obj.t, unit, unit) exportable)
+  =
+  fun fl ->
+    fun pi ->
+      fun mst ->
+        {
+          ityp = ();
+          c_ityp = (Obj.magic (Compiler_Languages.interm_bytes () () ()));
+          export =
+            (fun uu___1 ->
+               fun uu___ ->
+                 (fun uu___ ->
+                    fun b -> match uu___ with | Leaf -> Obj.magic b) uu___1
+                   uu___)
+        }
+let (exportable_refinement :
+  unit ->
+    unit ->
+      unit ->
+        unit pck_dc tree ->
+          unit ->
+            (Obj.t, unit, Obj.t, unit, unit) exportable ->
+              unit -> (Obj.t, unit, Obj.t, unit, unit) exportable)
+  =
+  fun fl ->
+    fun pi ->
+      fun mst ->
+        fun dcs ->
+          fun t ->
+            fun d ->
+              fun p ->
+                {
+                  ityp = ();
+                  c_ityp =
+                    (Obj.magic (interm_exportable_super () () () dcs d));
+                  export = (d.export)
+                }
+let (exportable_option :
+  unit ->
+    unit ->
+      unit ->
+        unit pck_dc tree ->
+          unit ->
+            (Obj.t, unit, Obj.t, unit, unit) exportable ->
+              (Obj.t FStar_Pervasives_Native.option, unit, Obj.t, unit, 
+                unit) exportable)
+  =
+  fun fl ->
+    fun pi ->
+      fun mst ->
+        fun dcs ->
+          fun t1 ->
+            fun d1 ->
+              {
+                ityp = ();
+                c_ityp =
+                  (Obj.magic
+                     (Compiler_Languages.interm_option () () () ()
+                        (Obj.magic (interm_exportable_super () () () dcs d1))));
+                export =
+                  (fun uu___1 ->
+                     fun uu___ ->
+                       (fun eff_dcs ->
+                          fun x ->
+                            match x with
+                            | FStar_Pervasives_Native.Some x' ->
+                                Obj.magic
+                                  (FStar_Pervasives_Native.Some
+                                     (d1.export eff_dcs x'))
+                            | FStar_Pervasives_Native.None ->
+                                Obj.magic FStar_Pervasives_Native.None)
+                         uu___1 uu___)
+              }
+let (exportable_pair :
+  unit ->
+    unit ->
+      unit ->
+        unit pck_dc tree ->
+          unit ->
+            (Obj.t, unit, Obj.t, unit, unit) exportable ->
+              unit ->
+                (Obj.t, unit, Obj.t, unit, unit) exportable ->
+                  ((Obj.t * Obj.t), unit, Obj.t, unit, unit) exportable)
+  =
+  fun fl ->
+    fun pi ->
+      fun mst ->
+        fun dcs ->
+          fun t1 ->
+            fun d1 ->
+              fun t2 ->
+                fun d2 ->
+                  {
+                    ityp = ();
+                    c_ityp =
+                      (Obj.magic
+                         (Compiler_Languages.interm_pair () () () ()
+                            (Obj.magic
+                               (interm_exportable_super () () () (left dcs)
+                                  d1)) ()
+                            (Obj.magic
+                               (interm_exportable_super () () () (right dcs)
+                                  d2))));
+                    export =
+                      (fun uu___1 ->
+                         fun uu___ ->
+                           (fun eff_dcs ->
+                              fun uu___ ->
+                                match uu___ with
+                                | (x, y) ->
+                                    Obj.magic
+                                      ((d1.export (left eff_dcs) x),
+                                        (d2.export (right eff_dcs) y)))
+                             uu___1 uu___)
+                  }
+let (exportable_either :
+  unit ->
+    unit ->
+      unit ->
+        unit pck_dc tree ->
+          unit ->
+            (Obj.t, unit, Obj.t, unit, unit) exportable ->
+              unit ->
+                (Obj.t, unit, Obj.t, unit, unit) exportable ->
+                  ((Obj.t, Obj.t) FStar_Pervasives.either, unit, Obj.t, 
+                    unit, unit) exportable)
+  =
+  fun fl ->
+    fun pi ->
+      fun mst ->
+        fun dcs ->
+          fun t1 ->
+            fun d1 ->
+              fun t2 ->
+                fun d2 ->
+                  {
+                    ityp = ();
+                    c_ityp =
+                      (Obj.magic
+                         (Compiler_Languages.interm_either () () () ()
+                            (Obj.magic
+                               (interm_exportable_super () () () (left dcs)
+                                  d1)) ()
+                            (Obj.magic
+                               (interm_exportable_super () () () (right dcs)
+                                  d2))));
+                    export =
+                      (fun uu___1 ->
+                         fun uu___ ->
+                           (fun eff_dcs ->
+                              fun x ->
+                                match x with
+                                | FStar_Pervasives.Inl x1 ->
+                                    Obj.magic
+                                      (FStar_Pervasives.Inl
+                                         (d1.export (left eff_dcs) x1))
+                                | FStar_Pervasives.Inr x1 ->
+                                    Obj.magic
+                                      (FStar_Pervasives.Inr
+                                         (d2.export (right eff_dcs) x1)))
+                             uu___1 uu___)
+                  }
+let (exportable_arrow_with_no_pre_and_no_post :
+  unit ->
+    unit ->
+      unit ->
+        unit pck_dc tree ->
+          unit ->
+            (Obj.t, unit, Obj.t, unit, unit) importable ->
+              unit ->
+                (Obj.t, unit, Obj.t, unit, unit) exportable ->
+                  (Obj.t ->
+                     (Obj.t CommonUtils.resexn, unit, unit, unit) MIO.dm_gmio,
+                    unit, Obj.t, unit, unit) exportable)
+  =
+  fun fl ->
+    fun pi ->
+      fun mst ->
+        fun dcs ->
+          fun t1 ->
+            fun d1 ->
+              fun t2 ->
+                fun d2 ->
+                  {
+                    ityp = ();
+                    c_ityp =
+                      (Obj.magic
+                         (Compiler_Languages.interm_arrow () () () ()
+                            (Obj.magic
+                               (interm_importable_super () () () (left dcs)
+                                  d1)) ()
+                            (Obj.magic
+                               (Compiler_Languages.interm_resexn () () () ()
+                                  (Obj.magic
+                                     (interm_exportable_super () () ()
+                                        (right dcs) d2))))));
+                    export =
+                      (fun uu___1 ->
+                         fun uu___ ->
+                           (fun eff_dcs ->
+                              fun f ->
+                                Obj.magic
+                                  (fun x ->
+                                     match d1.import x (left eff_dcs) with
+                                     | FStar_Pervasives.Inl x' ->
+                                         MIO.dm_gmio_bind () () () () ()
+                                           (Obj.magic (f x'))
+                                           (fun uu___ ->
+                                              match uu___ with
+                                              | FStar_Pervasives.Inl x'' ->
+                                                  MIO.lift_pure_dm_gmio () ()
+                                                    (fun uu___1 ->
+                                                       (fun uu___1 ->
+                                                          Obj.magic
+                                                            (FStar_Pervasives.Inl
+                                                               (d2.export
+                                                                  (right
+                                                                    eff_dcs)
+                                                                  x'')))
+                                                         uu___1)
+                                              | FStar_Pervasives.Inr err ->
+                                                  MIO.lift_pure_dm_gmio () ()
+                                                    (fun uu___1 ->
+                                                       (fun uu___1 ->
+                                                          Obj.magic
+                                                            (FStar_Pervasives.Inr
+                                                               err)) uu___1))
+                                     | FStar_Pervasives.Inr err ->
+                                         MIO.lift_pure_dm_gmio () ()
+                                           (fun uu___ ->
+                                              (fun uu___ ->
+                                                 Obj.magic
+                                                   (FStar_Pervasives.Inr err))
+                                                uu___))) uu___1 uu___)
+                  }
+let (exportable_arrow_post_args :
+  unit ->
+    unit ->
+      unit ->
+        unit pck_dc tree ->
+          unit ->
+            (Obj.t, unit, Obj.t, unit, unit) importable ->
+              unit ->
+                (Obj.t, unit, Obj.t, unit, unit) exportable ->
+                  unit ->
+                    unit ->
+                      (Obj.t ->
+                         (Obj.t CommonUtils.resexn, unit, unit, unit)
+                           MIO.dm_gmio,
+                        unit, Obj.t, unit, unit) exportable)
+  =
+  fun fl ->
+    fun pi ->
+      fun mst ->
+        fun dcs ->
+          fun t1 ->
+            fun d1 ->
+              fun t2 ->
+                fun d2 ->
+                  fun post ->
+                    fun c1 ->
+                      {
+                        ityp = ();
+                        c_ityp =
+                          (Obj.magic
+                             (Compiler_Languages.interm_arrow () () () ()
+                                (Obj.magic
+                                   (interm_importable_super () () ()
+                                      (left dcs) d1)) ()
+                                (Obj.magic
+                                   (Compiler_Languages.interm_resexn () () ()
+                                      ()
+                                      (Obj.magic
+                                         (interm_exportable_super () () ()
+                                            (right dcs) d2))))));
+                        export =
+                          (fun eff_dcs ->
+                             fun f ->
+                               let f' = f in
+                               (exportable_arrow_with_no_pre_and_no_post ()
+                                  () () dcs () d1 () d2).export eff_dcs f')
+                      }
+let (exportable_arrow_post :
+  unit ->
+    unit ->
+      unit ->
+        unit pck_dc tree ->
+          unit ->
+            (Obj.t, unit, Obj.t, unit, unit) importable ->
+              unit ->
+                (Obj.t, unit, Obj.t, unit, unit) exportable ->
+                  unit ->
+                    unit ->
+                      (Obj.t ->
+                         (Obj.t CommonUtils.resexn, unit, unit, unit)
+                           MIO.dm_gmio,
+                        unit, Obj.t, unit, unit) exportable)
+  =
+  fun fl ->
+    fun pi ->
+      fun mst ->
+        fun dcs ->
+          fun t1 ->
+            fun d1 ->
+              fun t2 ->
+                fun d2 ->
+                  fun post ->
+                    fun c1 ->
+                      exportable_arrow_post_args () () () dcs () d1 () d2 ()
+                        ()
+type ('a, 'b, 'pre, 'post, 'x, 'h, 'r, 'lt) trivialize_new_post = unit
+let enforce_pre :
+  't1 't2 .
+    unit ->
+      unit ->
+        unit ->
+          (unit, unit) idc_typ ->
+            (unit, unit, unit, unit) dc_typ ->
+              (unit, unit, unit, unit, unit, unit) eff_dc_typ ->
+                unit ->
+                  unit ->
+                    ('t1 ->
+                       ('t2 CommonUtils.resexn, unit, unit, unit) MIO.dm_gmio)
+                      ->
+                      't1 ->
+                        ('t2 CommonUtils.resexn, unit, unit, unit)
+                          MIO.dm_gmio
+  =
+  fun uu___9 ->
+    fun uu___8 ->
+      fun uu___7 ->
+        fun uu___6 ->
+          fun uu___5 ->
+            fun uu___4 ->
+              fun uu___3 ->
+                fun uu___2 ->
+                  fun uu___1 ->
+                    fun uu___ ->
+                      (fun fl ->
+                         fun mst ->
+                           fun pre ->
+                             fun idc ->
+                               fun dc ->
+                                 fun eff_dc ->
+                                   fun post ->
+                                     fun c_pre ->
+                                       fun f ->
+                                         fun x ->
+                                           Obj.magic
+                                             (MIO.dm_gmio_bind () () () () ()
+                                                (Obj.magic (eff_dc ()))
+                                                (fun uu___ ->
+                                                   match Obj.magic uu___ with
+                                                   | FStar_Pervasives.Mkdtuple3
+                                                       (uu___1, uu___2,
+                                                        eff_dc')
+                                                       ->
+                                                       MIO.dm_gmio_bind () ()
+                                                         () () ()
+                                                         (Obj.magic
+                                                            (eff_dc' ()))
+                                                         (fun uu___3 ->
+                                                            (fun uu___3 ->
+                                                               if uu___3
+                                                               then
+                                                                 Obj.magic
+                                                                   (Obj.repr
+                                                                    (f x))
+                                                               else
+                                                                 Obj.magic
+                                                                   (Obj.repr
+                                                                    (MIO.lift_pure_dm_gmio
+                                                                    () ()
+                                                                    (fun
+                                                                    uu___5 ->
+                                                                    FStar_Pervasives.Inr
+                                                                    CommonUtils.Contract_failure))))
+                                                              uu___3))))
+                        uu___9 uu___8 uu___7 uu___6 uu___5 uu___4 uu___3
+                        uu___2 uu___1 uu___
+let enforce_pre_args :
+  't1 't2 .
+    unit ->
+      unit ->
+        unit ->
+          ('t1, unit) idc_typ ->
+            (unit, 't1, unit, unit) dc_typ ->
+              (unit, unit, 't1, unit, unit, unit) eff_dc_typ ->
+                unit ->
+                  unit ->
+                    ('t1 ->
+                       ('t2 CommonUtils.resexn, unit, unit, unit) MIO.dm_gmio)
+                      ->
+                      't1 ->
+                        ('t2 CommonUtils.resexn, unit, unit, unit)
+                          MIO.dm_gmio
+  =
+  fun uu___9 ->
+    fun uu___8 ->
+      fun uu___7 ->
+        fun uu___6 ->
+          fun uu___5 ->
+            fun uu___4 ->
+              fun uu___3 ->
+                fun uu___2 ->
+                  fun uu___1 ->
+                    fun uu___ ->
+                      (fun fl ->
+                         fun mst ->
+                           fun pre ->
+                             fun idc ->
+                               fun dc ->
+                                 fun eff_dc ->
+                                   fun post ->
+                                     fun c_pre ->
+                                       fun f ->
+                                         fun x ->
+                                           Obj.magic
+                                             (MIO.dm_gmio_bind () () () () ()
+                                                (Obj.magic (eff_dc x))
+                                                (fun uu___ ->
+                                                   match Obj.magic uu___ with
+                                                   | FStar_Pervasives.Mkdtuple3
+                                                       (uu___1, uu___2,
+                                                        eff_dc')
+                                                       ->
+                                                       MIO.dm_gmio_bind () ()
+                                                         () () ()
+                                                         (Obj.magic
+                                                            (eff_dc' ()))
+                                                         (fun uu___3 ->
+                                                            (fun uu___3 ->
+                                                               if uu___3
+                                                               then
+                                                                 Obj.magic
+                                                                   (Obj.repr
+                                                                    (f x))
+                                                               else
+                                                                 Obj.magic
+                                                                   (Obj.repr
+                                                                    (MIO.lift_pure_dm_gmio
+                                                                    () ()
+                                                                    (fun
+                                                                    uu___5 ->
+                                                                    FStar_Pervasives.Inr
+                                                                    CommonUtils.Contract_failure))))
+                                                              uu___3))))
+                        uu___9 uu___8 uu___7 uu___6 uu___5 uu___4 uu___3
+                        uu___2 uu___1 uu___
+let rityp_idc : 'a 'b 'c 'd . ('a, 'b) idc_typ -> ('c, 'd) idc_typ =
+  fun uu___ -> (fun idc -> Obj.magic idc) uu___
+let (rityp_eff_dc :
+  unit ->
+    unit ->
+      unit ->
+        unit ->
+          unit ->
+            unit ->
+              (Obj.t, Obj.t) idc_typ ->
+                (unit, Obj.t, Obj.t, unit) dc_typ ->
+                  (unit, unit, Obj.t, Obj.t, unit, unit) eff_dc_typ ->
+                    (unit, unit, Obj.t, Obj.t, unit, unit) eff_dc_typ)
+  =
+  fun uu___8 ->
+    fun uu___7 ->
+      fun uu___6 ->
+        fun uu___5 ->
+          fun uu___4 ->
+            fun uu___3 ->
+              fun uu___2 ->
+                fun uu___1 ->
+                  fun uu___ ->
+                    (fun mst ->
+                       fun fl ->
+                         fun a ->
+                           fun b ->
+                             fun c ->
+                               fun d ->
+                                 fun idc ->
+                                   fun dc ->
+                                     fun eff_dc ->
+                                       Obj.magic
+                                         (fun x ->
+                                            MIO.dm_gmio_bind () () () () ()
+                                              (Obj.magic (eff_dc x))
+                                              (fun uu___ ->
+                                                 MIO.lift_pure_dm_gmio () ()
+                                                   (fun uu___1 ->
+                                                      (fun uu___1 ->
+                                                         match Obj.magic
+                                                                 uu___
+                                                         with
+                                                         | FStar_Pervasives.Mkdtuple3
+                                                             (s0, h0, cont)
+                                                             ->
+                                                             Obj.magic
+                                                               (FStar_Pervasives.Mkdtuple3
+                                                                  (s0, (),
+                                                                    (
+                                                                    fun y ->
+                                                                    cont y))))
+                                                        uu___1)))) uu___8
+                      uu___7 uu___6 uu___5 uu___4 uu___3 uu___2 uu___1 uu___
+let exportable_arrow_pre_post_args :
+  't1 't2 .
+    unit ->
+      unit ->
+        unit ->
+          unit pck_dc tree ->
+            ('t1, unit, Obj.t, unit, unit) importable ->
+              ('t2, unit, Obj.t, unit, unit) exportable ->
+                unit ->
+                  unit ->
+                    unit ->
+                      unit ->
+                        ('t1 ->
+                           ('t2 CommonUtils.resexn, unit, unit, unit)
+                             MIO.dm_gmio,
+                          unit, Obj.t, unit, unit) exportable
+  =
+  fun fl ->
+    fun pi ->
+      fun mst ->
+        fun dcs ->
+          fun d1 ->
+            fun d2 ->
+              fun pre ->
+                fun post ->
+                  fun c_pre ->
+                    fun c1 ->
+                      {
+                        ityp = ();
+                        c_ityp =
+                          (Obj.magic
+                             (Compiler_Languages.interm_arrow () () () ()
+                                (Obj.magic
+                                   (interm_importable_super () () ()
+                                      (left dcs) d1)) ()
+                                (Obj.magic
+                                   (Compiler_Languages.interm_resexn () () ()
+                                      ()
+                                      (Obj.magic
+                                         (interm_exportable_super () () ()
+                                            (right dcs) d2))))));
+                        export =
+                          (fun eff_dcs ->
+                             fun f ->
+                               let uu___ = root eff_dcs in
+                               match uu___ with
+                               | Prims.Mkdtuple2
+                                   (FStar_Pervasives.Mkdtuple4
+                                    (a, b, idc, dc), eff_dc)
+                                   ->
+                                   let eff_dc1 =
+                                     Obj.magic
+                                       (rityp_eff_dc () () () () () ()
+                                          (FStar_Pervasives.__proj__Mkdtuple4__item___3
+                                             (FStar_Pervasives.Mkdtuple4
+                                                ((), (), idc, dc)))
+                                          (FStar_Pervasives.__proj__Mkdtuple4__item___4
+                                             (FStar_Pervasives.Mkdtuple4
+                                                ((), (), idc, dc)))
+                                          (Obj.magic eff_dc)) in
+                                   let f' =
+                                     enforce_pre_args () () ()
+                                       (rityp_idc
+                                          (FStar_Pervasives.__proj__Mkdtuple4__item___3
+                                             (FStar_Pervasives.Mkdtuple4
+                                                ((), (), idc, dc))))
+                                       (Obj.magic dc) eff_dc1 () () f in
+                                   let dc_pre x h = idc x h (Obj.repr ()) [] in
+                                   let dcs' =
+                                     EmptyNode ((left dcs), (right dcs)) in
+                                   let eff_dcs' =
+                                     EmptyNode
+                                       ((left eff_dcs), (right eff_dcs)) in
+                                   let d uu___1 =
+                                     (Obj.magic
+                                        (exportable_arrow_post_args () () ()
+                                           dcs' () (Obj.magic d1) ()
+                                           (Obj.magic d2) ())) uu___1 in
+                                   (d ()).export eff_dcs' f')
+                      }
+let exportable_arrow_pre_post :
+  't1 't2 .
+    unit ->
+      unit ->
+        unit ->
+          unit pck_dc tree ->
+            ('t1, unit, Obj.t, unit, unit) importable ->
+              ('t2, unit, Obj.t, unit, unit) exportable ->
+                unit ->
+                  unit ->
+                    unit ->
+                      unit ->
+                        ('t1 ->
+                           ('t2 CommonUtils.resexn, unit, unit, unit)
+                             MIO.dm_gmio,
+                          unit, Obj.t, unit, unit) exportable
+  =
+  fun fl ->
+    fun pi ->
+      fun mst ->
+        fun dcs ->
+          fun d1 ->
+            fun d2 ->
+              fun pre ->
+                fun post ->
+                  fun c_pre ->
+                    fun c1 ->
+                      {
+                        ityp = ();
+                        c_ityp =
+                          (Obj.magic
+                             (Compiler_Languages.interm_arrow () () () ()
+                                (Obj.magic
+                                   (interm_importable_super () () ()
+                                      (left dcs) d1)) ()
+                                (Obj.magic
+                                   (Compiler_Languages.interm_resexn () () ()
+                                      ()
+                                      (Obj.magic
+                                         (interm_exportable_super () () ()
+                                            (right dcs) d2))))));
+                        export =
+                          (fun eff_dcs ->
+                             fun f ->
+                               let uu___ = root eff_dcs in
+                               match uu___ with
+                               | Prims.Mkdtuple2
+                                   (FStar_Pervasives.Mkdtuple4
+                                    (a, b, idc, dc), eff_dc)
+                                   ->
+                                   let eff_dc1 =
+                                     Obj.magic
+                                       (rityp_eff_dc () () () () () ()
+                                          (FStar_Pervasives.__proj__Mkdtuple4__item___3
+                                             (FStar_Pervasives.Mkdtuple4
+                                                ((), (), idc, dc)))
+                                          (FStar_Pervasives.__proj__Mkdtuple4__item___4
+                                             (FStar_Pervasives.Mkdtuple4
+                                                ((), (), idc, dc)))
+                                          (Obj.magic eff_dc)) in
+                                   let f' =
+                                     enforce_pre () () ()
+                                       (rityp_idc
+                                          (FStar_Pervasives.__proj__Mkdtuple4__item___3
+                                             (FStar_Pervasives.Mkdtuple4
+                                                ((), (), idc, dc))))
+                                       (Obj.magic dc) eff_dc1 () () f in
+                                   let dc_pre x h =
+                                     idc (Obj.repr ()) h (Obj.repr ()) [] in
+                                   let dcs' =
+                                     EmptyNode ((left dcs), (right dcs)) in
+                                   let eff_dcs' =
+                                     EmptyNode
+                                       ((left eff_dcs), (right eff_dcs)) in
+                                   let d uu___1 =
+                                     (Obj.magic
+                                        (exportable_arrow_post_args () () ()
+                                           dcs' () (Obj.magic d1) ()
+                                           (Obj.magic d2) ())) uu___1 in
+                                   (d ()).export eff_dcs' f')
+                      }
+let (interm_is_safely_importable :
+  unit ->
+    unit ->
+      unit ->
+        unit pck_dc tree ->
+          unit ->
+            (Obj.t, unit, Obj.t, unit) Compiler_Languages.interm ->
+              (Obj.t, unit, Obj.t, unit, unit) safe_importable)
+  =
+  fun fl ->
+    fun pi ->
+      fun mst ->
+        fun dcs ->
+          fun t ->
+            fun d ->
+              {
+                ityp1 = ();
+                c_ityp1 = d;
+                safe_import =
+                  (fun x -> fun uu___ -> match uu___ with | Leaf -> x)
+              }
+let (importable_unit :
+  unit -> unit -> unit -> (unit, unit, Obj.t, unit, unit) importable) =
+  fun fl ->
+    fun pi ->
+      fun mst ->
+        {
+          ityp2 = ();
+          c_ityp2 = (Obj.magic (Compiler_Languages.interm_unit () () ()));
+          import =
+            (fun uu___1 ->
+               fun uu___ ->
+                 (fun uu___ ->
+                    let uu___ = Obj.magic uu___ in
+                    fun uu___1 ->
+                      match uu___1 with
+                      | Leaf -> Obj.magic (FStar_Pervasives.Inl ())) uu___1
+                   uu___)
+        }
+let (importable_file_descr :
+  unit ->
+    unit ->
+      unit -> (UnixTypes.file_descr, unit, Obj.t, unit, unit) importable)
+  =
+  fun fl ->
+    fun pi ->
+      fun mst ->
+        {
+          ityp2 = ();
+          c_ityp2 = (Obj.magic (Compiler_Languages.interm_int () () ()));
+          import =
+            (fun uu___1 ->
+               fun uu___ ->
+                 (fun fd ->
+                    let fd = Obj.magic fd in
+                    fun uu___ ->
+                      match uu___ with
+                      | Leaf -> Obj.magic (FStar_Pervasives.Inl fd)) uu___1
+                   uu___)
+        }
+let (importable_bytes :
+  unit ->
+    unit -> unit -> (FStar_Bytes.bytes, unit, Obj.t, unit, unit) importable)
+  =
+  fun fl ->
+    fun pi ->
+      fun mst ->
+        {
+          ityp2 = ();
+          c_ityp2 = (Obj.magic (Compiler_Languages.interm_bytes () () ()));
+          import =
+            (fun uu___1 ->
+               fun uu___ ->
+                 (fun b ->
+                    let b = Obj.magic b in
+                    fun uu___ ->
+                      match uu___ with
+                      | Leaf -> Obj.magic (FStar_Pervasives.Inl b)) uu___1
+                   uu___)
+        }
+let (safe_importable_is_importable :
+  unit ->
+    unit ->
+      unit ->
+        unit pck_dc tree ->
+          unit ->
+            (Obj.t, unit, Obj.t, unit, unit) safe_importable ->
+              (Obj.t, unit, Obj.t, unit, unit) importable)
+  =
+  fun fl ->
+    fun pi ->
+      fun mst ->
+        fun dcs ->
+          fun t ->
+            fun d ->
+              {
+                ityp2 = ();
+                c_ityp2 =
+                  (Obj.magic (interm_safe_importable_super () () () dcs d));
+                import =
+                  (fun x ->
+                     fun eff_dcs ->
+                       FStar_Pervasives.Inl (d.safe_import x eff_dcs))
+              }
+let (importable_refinement :
+  unit ->
+    unit ->
+      unit ->
+        unit pck_dc tree ->
+          unit ->
+            (Obj.t, unit, Obj.t, unit, unit) importable ->
+              unit ->
+                (Obj.t, Obj.t) TC_Checkable.checkable ->
+                  (Obj.t, unit, Obj.t, unit, unit) importable)
+  =
+  fun fl ->
+    fun pi ->
+      fun mst ->
+        fun dcs ->
+          fun t ->
+            fun d ->
+              fun rp ->
+                fun d1 ->
+                  {
+                    ityp2 = ();
+                    c_ityp2 =
+                      (Obj.magic (interm_importable_super () () () dcs d));
+                    import =
+                      (fun x ->
+                         fun eff_dcs ->
+                           match d.import x eff_dcs with
+                           | FStar_Pervasives.Inl x1 ->
+                               if d1.TC_Checkable.check x1
+                               then FStar_Pervasives.Inl x1
+                               else
+                                 FStar_Pervasives.Inr
+                                   CommonUtils.Contract_failure
+                           | FStar_Pervasives.Inr err ->
+                               FStar_Pervasives.Inr err)
+                  }
+let (importable_option :
+  unit ->
+    unit ->
+      unit ->
+        unit pck_dc tree ->
+          unit ->
+            (Obj.t, unit, Obj.t, unit, unit) importable ->
+              (Obj.t FStar_Pervasives_Native.option, unit, Obj.t, unit, 
+                unit) importable)
+  =
+  fun fl ->
+    fun pi ->
+      fun mst ->
+        fun dcs ->
+          fun t ->
+            fun d ->
+              {
+                ityp2 = ();
+                c_ityp2 =
+                  (Obj.magic
+                     (Compiler_Languages.interm_option () () () ()
+                        (Obj.magic (interm_importable_super () () () dcs d))));
+                import =
+                  (fun uu___1 ->
+                     fun uu___ ->
+                       (fun x ->
+                          let x = Obj.magic x in
+                          fun eff_dcs ->
+                            match Obj.magic x with
+                            | FStar_Pervasives_Native.Some x' ->
+                                (match d.import x' eff_dcs with
+                                 | FStar_Pervasives.Inl x'' ->
+                                     Obj.magic
+                                       (FStar_Pervasives.Inl
+                                          (FStar_Pervasives_Native.Some x''))
+                                 | FStar_Pervasives.Inr err ->
+                                     Obj.magic (FStar_Pervasives.Inr err))
+                            | FStar_Pervasives_Native.None ->
+                                Obj.magic
+                                  (FStar_Pervasives.Inr
+                                     CommonUtils.Contract_failure)) uu___1
+                         uu___)
+              }
+let (importable_pair :
+  unit ->
+    unit ->
+      unit ->
+        unit pck_dc tree ->
+          unit ->
+            unit ->
+              (Obj.t, unit, Obj.t, unit, unit) importable ->
+                (Obj.t, unit, Obj.t, unit, unit) importable ->
+                  ((Obj.t * Obj.t), unit, Obj.t, unit, unit) importable)
+  =
+  fun fl ->
+    fun pi ->
+      fun mst ->
+        fun dcs ->
+          fun t1 ->
+            fun t2 ->
+              fun d1 ->
+                fun d2 ->
+                  {
+                    ityp2 = ();
+                    c_ityp2 =
+                      (Obj.magic
+                         (Compiler_Languages.interm_pair () () () ()
+                            (Obj.magic
+                               (interm_importable_super () () () (left dcs)
+                                  d1)) ()
+                            (Obj.magic
+                               (interm_importable_super () () () (right dcs)
+                                  d2))));
+                    import =
+                      (fun uu___1 ->
+                         fun uu___ ->
+                           (fun uu___ ->
+                              let uu___ = Obj.magic uu___ in
+                              fun eff_dcs ->
+                                match Obj.magic uu___ with
+                                | (x, y) ->
+                                    (match ((d1.import x (left eff_dcs)),
+                                             (d2.import y (right eff_dcs)))
+                                     with
+                                     | (FStar_Pervasives.Inl x1,
+                                        FStar_Pervasives.Inl y1) ->
+                                         Obj.magic
+                                           (FStar_Pervasives.Inl (x1, y1))
+                                     | uu___1 ->
+                                         Obj.magic
+                                           (FStar_Pervasives.Inr
+                                              CommonUtils.Contract_failure)))
+                             uu___1 uu___)
+                  }
+let (importable_either :
+  unit ->
+    unit ->
+      unit ->
+        unit pck_dc tree ->
+          unit ->
+            unit ->
+              (Obj.t, unit, Obj.t, unit, unit) importable ->
+                (Obj.t, unit, Obj.t, unit, unit) importable ->
+                  ((Obj.t, Obj.t) FStar_Pervasives.either, unit, Obj.t, 
+                    unit, unit) importable)
+  =
+  fun fl ->
+    fun pi ->
+      fun mst ->
+        fun dcs ->
+          fun t1 ->
+            fun t2 ->
+              fun d1 ->
+                fun d2 ->
+                  {
+                    ityp2 = ();
+                    c_ityp2 =
+                      (Obj.magic
+                         (Compiler_Languages.interm_either () () () ()
+                            (Obj.magic
+                               (interm_importable_super () () () (left dcs)
+                                  d1)) ()
+                            (Obj.magic
+                               (interm_importable_super () () () (right dcs)
+                                  d2))));
+                    import =
+                      (fun uu___1 ->
+                         fun uu___ ->
+                           (fun x ->
+                              let x = Obj.magic x in
+                              fun eff_dcs ->
+                                match Obj.magic x with
+                                | FStar_Pervasives.Inl x' ->
+                                    (match d1.import x' (left eff_dcs) with
+                                     | FStar_Pervasives.Inl x'' ->
+                                         Obj.magic
+                                           (FStar_Pervasives.Inl
+                                              (FStar_Pervasives.Inl x''))
+                                     | FStar_Pervasives.Inr err ->
+                                         Obj.magic (FStar_Pervasives.Inr err))
+                                | FStar_Pervasives.Inr y ->
+                                    (match d2.import y (right eff_dcs) with
+                                     | FStar_Pervasives.Inl y' ->
+                                         Obj.magic
+                                           (FStar_Pervasives.Inl
+                                              (FStar_Pervasives.Inr y'))
+                                     | FStar_Pervasives.Inr err ->
+                                         Obj.magic (FStar_Pervasives.Inr err)))
+                             uu___1 uu___)
+                  }
+let (importable_dpair_refined :
+  unit ->
+    unit ->
+      unit ->
+        unit pck_dc tree ->
+          unit ->
+            unit ->
+              unit ->
+                (Obj.t, unit, Obj.t, unit, unit) importable ->
+                  (Obj.t, unit, Obj.t, unit, unit) importable ->
+                    (Obj.t, Obj.t, Obj.t) TC_Checkable.checkable2 ->
+                      ((Obj.t, Obj.t) Prims.dtuple2, unit, Obj.t, unit, 
+                        unit) importable)
+  =
+  fun fl ->
+    fun pi ->
+      fun mst ->
+        fun dcs ->
+          fun t1 ->
+            fun t2 ->
+              fun p ->
+                fun d1 ->
+                  fun d2 ->
+                    fun d3 ->
+                      {
+                        ityp2 = ();
+                        c_ityp2 =
+                          (Obj.magic
+                             (Compiler_Languages.interm_pair () () () ()
+                                (Obj.magic
+                                   (interm_importable_super () () ()
+                                      (left dcs) d1)) ()
+                                (Obj.magic
+                                   (interm_importable_super () () ()
+                                      (right dcs) d2))));
+                        import =
+                          (fun uu___1 ->
+                             fun uu___ ->
+                               (fun uu___ ->
+                                  let uu___ = Obj.magic uu___ in
+                                  fun eff_dcs ->
+                                    match Obj.magic uu___ with
+                                    | (x', y') ->
+                                        (match ((d1.import x' (left eff_dcs)),
+                                                 (d2.import y'
+                                                    (right eff_dcs)))
+                                         with
+                                         | (FStar_Pervasives.Inl x,
+                                            FStar_Pervasives.Inl y) ->
+                                             if
+                                               TC_Checkable.check2 () () d3 x
+                                                 y
+                                             then
+                                               Obj.magic
+                                                 (FStar_Pervasives.Inl
+                                                    (Prims.Mkdtuple2 (x, y)))
+                                             else
+                                               Obj.magic
+                                                 (FStar_Pervasives.Inr
+                                                    CommonUtils.Contract_failure)
+                                         | uu___1 ->
+                                             Obj.magic
+                                               (FStar_Pervasives.Inr
+                                                  CommonUtils.Contract_failure)))
+                                 uu___1 uu___)
+                      }
+let (safe_importable_resexn :
+  unit ->
+    unit ->
+      unit ->
+        unit pck_dc tree ->
+          unit ->
+            (Obj.t, unit, Obj.t, unit, unit) importable ->
+              (Obj.t CommonUtils.resexn, unit, Obj.t, unit, unit)
+                safe_importable)
+  =
+  fun fl ->
+    fun pi ->
+      fun mst ->
+        fun dcs ->
+          fun t1 ->
+            fun d1 ->
+              {
+                ityp1 = ();
+                c_ityp1 =
+                  (Obj.magic
+                     (Compiler_Languages.interm_resexn () () () ()
+                        (Obj.magic (interm_importable_super () () () dcs d1))));
+                safe_import =
+                  (fun uu___1 ->
+                     fun uu___ ->
+                       (fun x ->
+                          let x = Obj.magic x in
+                          fun eff_dcs ->
+                            match Obj.magic x with
+                            | FStar_Pervasives.Inl x' ->
+                                Obj.magic (d1.import x' eff_dcs)
+                            | FStar_Pervasives.Inr y ->
+                                Obj.magic (FStar_Pervasives.Inr y)) uu___1
+                         uu___)
+              }
+let (safe_importable_arrow :
+  unit ->
+    unit ->
+      unit ->
+        unit pck_dc tree ->
+          unit ->
+            (Obj.t, unit, Obj.t, unit, unit) exportable ->
+              unit ->
+                (Obj.t, unit, Obj.t, unit, unit) importable ->
+                  (Obj.t ->
+                     (Obj.t CommonUtils.resexn, unit, unit, unit) MIO.dm_gmio,
+                    unit, Obj.t, unit, unit) safe_importable)
+  =
+  fun fl ->
+    fun pi ->
+      fun mst ->
+        fun dcs ->
+          fun t1 ->
+            fun d1 ->
+              fun t2 ->
+                fun d2 ->
+                  {
+                    ityp1 = ();
+                    c_ityp1 =
+                      (Obj.magic
+                         (Compiler_Languages.interm_arrow () () () ()
+                            (Obj.magic
+                               (interm_exportable_super () () () (left dcs)
+                                  d1)) ()
+                            (Obj.magic
+                               (Compiler_Languages.interm_resexn () () () ()
+                                  (Obj.magic
+                                     (interm_importable_super () () ()
+                                        (right dcs) d2))))));
+                    safe_import =
+                      (fun uu___2 ->
+                         fun uu___1 ->
+                           fun uu___ ->
+                             (fun f ->
+                                let f = Obj.magic f in
+                                fun eff_dcs ->
+                                  fun x ->
+                                    Obj.magic
+                                      (MIO.dm_gmio_bind () () () () ()
+                                         (MIO.lift_pure_dm_gmio () ()
+                                            (fun uu___ ->
+                                               d1.export (left eff_dcs) x))
+                                         (fun x' ->
+                                            MIO.dm_gmio_bind () () () () ()
+                                              (Obj.magic (f x'))
+                                              (fun y ->
+                                                 MIO.lift_pure_dm_gmio () ()
+                                                   (fun uu___ ->
+                                                      (safe_importable_resexn
+                                                         () () () (right dcs)
+                                                         () d2).safe_import
+                                                        (Obj.magic y)
+                                                        (right eff_dcs))))))
+                               uu___2 uu___1 uu___)
+                  }
+let enforce_post_args_res :
+  't1 't2 .
+    unit ->
+      unit ->
+        unit ->
+          unit ->
+            unit ->
+              ('t1, 't2 CommonUtils.resexn) idc_typ ->
+                (unit, 't1, 't2 CommonUtils.resexn, unit) dc_typ ->
+                  (unit, unit, 't1, 't2 CommonUtils.resexn, unit, unit)
+                    eff_dc_typ ->
+                    unit ->
+                      unit ->
+                        ('t1 ->
+                           ('t2 CommonUtils.resexn, unit, unit, unit)
+                             MIO.dm_gmio)
+                          ->
+                          't1 ->
+                            ('t2 CommonUtils.resexn, unit, unit, unit)
+                              MIO.dm_gmio
+  =
+  fun uu___11 ->
+    fun uu___10 ->
+      fun uu___9 ->
+        fun uu___8 ->
+          fun uu___7 ->
+            fun uu___6 ->
+              fun uu___5 ->
+                fun uu___4 ->
+                  fun uu___3 ->
+                    fun uu___2 ->
+                      fun uu___1 ->
+                        fun uu___ ->
+                          (fun fl ->
+                             fun pi ->
+                               fun mst ->
+                                 fun pre ->
+                                   fun post ->
+                                     fun idc ->
+                                       fun dc ->
+                                         fun eff_dc ->
+                                           fun c1post ->
+                                             fun c2post ->
+                                               fun f ->
+                                                 fun x ->
+                                                   Obj.magic
+                                                     (MIO.dm_gmio_bind () ()
+                                                        () () ()
+                                                        (Obj.magic (eff_dc x))
+                                                        (fun uu___ ->
+                                                           match Obj.magic
+                                                                   uu___
+                                                           with
+                                                           | FStar_Pervasives.Mkdtuple3
+                                                               (s0, h,
+                                                                eff_dc')
+                                                               ->
+                                                               MIO.dm_gmio_bind
+                                                                 () () () ()
+                                                                 ()
+                                                                 (Obj.magic
+                                                                    (
+                                                                    f x))
+                                                                 (fun r ->
+                                                                    MIO.dm_gmio_bind
+                                                                    () () ()
+                                                                    () ()
+                                                                    (Obj.magic
+                                                                    (eff_dc'
+                                                                    r))
+                                                                    (fun
+                                                                    uu___1 ->
+                                                                    if uu___1
+                                                                    then
+                                                                    MIO.lift_pure_dm_gmio
+                                                                    () ()
+                                                                    (fun
+                                                                    uu___2 ->
+                                                                    r)
+                                                                    else
+                                                                    MIO.lift_pure_dm_gmio
+                                                                    () ()
+                                                                    (fun
+                                                                    uu___3 ->
+                                                                    FStar_Pervasives.Inr
+                                                                    CommonUtils.Contract_failure))))))
+                            uu___11 uu___10 uu___9 uu___8 uu___7 uu___6
+                            uu___5 uu___4 uu___3 uu___2 uu___1 uu___
+let enforce_post_args :
+  't1 't2 .
+    unit ->
+      unit ->
+        unit ->
+          unit ->
+            unit ->
+              ('t1, unit) idc_typ ->
+                (unit, 't1, unit, unit) dc_typ ->
+                  (unit, unit, 't1, unit, unit, unit) eff_dc_typ ->
+                    unit ->
+                      unit ->
+                        ('t1 ->
+                           ('t2 CommonUtils.resexn, unit, unit, unit)
+                             MIO.dm_gmio)
+                          ->
+                          't1 ->
+                            ('t2 CommonUtils.resexn, unit, unit, unit)
+                              MIO.dm_gmio
+  =
+  fun uu___11 ->
+    fun uu___10 ->
+      fun uu___9 ->
+        fun uu___8 ->
+          fun uu___7 ->
+            fun uu___6 ->
+              fun uu___5 ->
+                fun uu___4 ->
+                  fun uu___3 ->
+                    fun uu___2 ->
+                      fun uu___1 ->
+                        fun uu___ ->
+                          (fun fl ->
+                             fun pi ->
+                               fun mst ->
+                                 fun pre ->
+                                   fun post ->
+                                     fun idc ->
+                                       fun dc ->
+                                         fun eff_dc ->
+                                           fun c1post ->
+                                             fun c2post ->
+                                               fun f ->
+                                                 fun x ->
+                                                   Obj.magic
+                                                     (MIO.dm_gmio_bind () ()
+                                                        () () ()
+                                                        (Obj.magic (eff_dc x))
+                                                        (fun uu___ ->
+                                                           match Obj.magic
+                                                                   uu___
+                                                           with
+                                                           | FStar_Pervasives.Mkdtuple3
+                                                               (uu___1, h,
+                                                                eff_dc')
+                                                               ->
+                                                               MIO.dm_gmio_bind
+                                                                 () () () ()
+                                                                 ()
+                                                                 (Obj.magic
+                                                                    (
+                                                                    f x))
+                                                                 (fun r ->
+                                                                    MIO.dm_gmio_bind
+                                                                    () () ()
+                                                                    () ()
+                                                                    (Obj.magic
+                                                                    (eff_dc'
+                                                                    ()))
+                                                                    (fun
+                                                                    uu___2 ->
+                                                                    if uu___2
+                                                                    then
+                                                                    MIO.lift_pure_dm_gmio
+                                                                    () ()
+                                                                    (fun
+                                                                    uu___3 ->
+                                                                    r)
+                                                                    else
+                                                                    MIO.lift_pure_dm_gmio
+                                                                    () ()
+                                                                    (fun
+                                                                    uu___4 ->
+                                                                    FStar_Pervasives.Inr
+                                                                    CommonUtils.Contract_failure))))))
+                            uu___11 uu___10 uu___9 uu___8 uu___7 uu___6
+                            uu___5 uu___4 uu___3 uu___2 uu___1 uu___
+let enforce_post_res :
+  't1 't2 .
+    unit ->
+      unit ->
+        unit ->
+          unit ->
+            unit ->
+              (unit, 't2 CommonUtils.resexn) idc_typ ->
+                (unit, unit, 't2 CommonUtils.resexn, unit) dc_typ ->
+                  (unit, unit, unit, 't2 CommonUtils.resexn, unit, unit)
+                    eff_dc_typ ->
+                    unit ->
+                      unit ->
+                        ('t1 ->
+                           ('t2 CommonUtils.resexn, unit, unit, unit)
+                             MIO.dm_gmio)
+                          ->
+                          't1 ->
+                            ('t2 CommonUtils.resexn, unit, unit, unit)
+                              MIO.dm_gmio
+  =
+  fun uu___11 ->
+    fun uu___10 ->
+      fun uu___9 ->
+        fun uu___8 ->
+          fun uu___7 ->
+            fun uu___6 ->
+              fun uu___5 ->
+                fun uu___4 ->
+                  fun uu___3 ->
+                    fun uu___2 ->
+                      fun uu___1 ->
+                        fun uu___ ->
+                          (fun fl ->
+                             fun pi ->
+                               fun mst ->
+                                 fun pre ->
+                                   fun post ->
+                                     fun idc ->
+                                       fun dc ->
+                                         fun eff_dc ->
+                                           fun c1post ->
+                                             fun c2post ->
+                                               fun f ->
+                                                 fun x ->
+                                                   Obj.magic
+                                                     (MIO.dm_gmio_bind () ()
+                                                        () () ()
+                                                        (Obj.magic
+                                                           (eff_dc ()))
+                                                        (fun uu___ ->
+                                                           match Obj.magic
+                                                                   uu___
+                                                           with
+                                                           | FStar_Pervasives.Mkdtuple3
+                                                               (uu___1, h,
+                                                                eff_dc')
+                                                               ->
+                                                               MIO.dm_gmio_bind
+                                                                 () () () ()
+                                                                 ()
+                                                                 (Obj.magic
+                                                                    (
+                                                                    f x))
+                                                                 (fun r ->
+                                                                    MIO.dm_gmio_bind
+                                                                    () () ()
+                                                                    () ()
+                                                                    (Obj.magic
+                                                                    (eff_dc'
+                                                                    r))
+                                                                    (fun
+                                                                    uu___2 ->
+                                                                    if uu___2
+                                                                    then
+                                                                    MIO.lift_pure_dm_gmio
+                                                                    () ()
+                                                                    (fun
+                                                                    uu___3 ->
+                                                                    r)
+                                                                    else
+                                                                    MIO.lift_pure_dm_gmio
+                                                                    () ()
+                                                                    (fun
+                                                                    uu___4 ->
+                                                                    FStar_Pervasives.Inr
+                                                                    CommonUtils.Contract_failure))))))
+                            uu___11 uu___10 uu___9 uu___8 uu___7 uu___6
+                            uu___5 uu___4 uu___3 uu___2 uu___1 uu___
+let enforce_post :
+  't1 't2 .
+    unit ->
+      unit ->
+        unit ->
+          unit ->
+            unit ->
+              (unit, unit) idc_typ ->
+                (unit, unit, unit, unit) dc_typ ->
+                  (unit, unit, unit, unit, unit, unit) eff_dc_typ ->
+                    unit ->
+                      unit ->
+                        ('t1 ->
+                           ('t2 CommonUtils.resexn, unit, unit, unit)
+                             MIO.dm_gmio)
+                          ->
+                          't1 ->
+                            ('t2 CommonUtils.resexn, unit, unit, unit)
+                              MIO.dm_gmio
+  =
+  fun uu___11 ->
+    fun uu___10 ->
+      fun uu___9 ->
+        fun uu___8 ->
+          fun uu___7 ->
+            fun uu___6 ->
+              fun uu___5 ->
+                fun uu___4 ->
+                  fun uu___3 ->
+                    fun uu___2 ->
+                      fun uu___1 ->
+                        fun uu___ ->
+                          (fun fl ->
+                             fun pi ->
+                               fun mst ->
+                                 fun pre ->
+                                   fun post ->
+                                     fun idc ->
+                                       fun dc ->
+                                         fun eff_dc ->
+                                           fun c1post ->
+                                             fun c2post ->
+                                               fun f ->
+                                                 fun x ->
+                                                   Obj.magic
+                                                     (MIO.dm_gmio_bind () ()
+                                                        () () ()
+                                                        (Obj.magic
+                                                           (eff_dc ()))
+                                                        (fun uu___ ->
+                                                           match Obj.magic
+                                                                   uu___
+                                                           with
+                                                           | FStar_Pervasives.Mkdtuple3
+                                                               (uu___1, h,
+                                                                eff_dc')
+                                                               ->
+                                                               MIO.dm_gmio_bind
+                                                                 () () () ()
+                                                                 ()
+                                                                 (Obj.magic
+                                                                    (
+                                                                    f x))
+                                                                 (fun r ->
+                                                                    MIO.dm_gmio_bind
+                                                                    () () ()
+                                                                    () ()
+                                                                    (Obj.magic
+                                                                    (eff_dc'
+                                                                    ()))
+                                                                    (fun
+                                                                    uu___2 ->
+                                                                    if uu___2
+                                                                    then
+                                                                    MIO.lift_pure_dm_gmio
+                                                                    () ()
+                                                                    (fun
+                                                                    uu___3 ->
+                                                                    r)
+                                                                    else
+                                                                    MIO.lift_pure_dm_gmio
+                                                                    () ()
+                                                                    (fun
+                                                                    uu___4 ->
+                                                                    FStar_Pervasives.Inr
+                                                                    CommonUtils.Contract_failure))))))
+                            uu___11 uu___10 uu___9 uu___8 uu___7 uu___6
+                            uu___5 uu___4 uu___3 uu___2 uu___1 uu___
+let safe_importable_arrow_pre_post_args_res :
+  't1 't2 .
+    unit ->
+      unit ->
+        unit ->
+          unit pck_dc tree ->
+            unit ->
+              unit ->
+                unit ->
+                  unit ->
+                    ('t1, unit, Obj.t, unit, unit) exportable ->
+                      ('t2, unit, Obj.t, unit, unit) importable ->
+                        ('t1 ->
+                           ('t2 CommonUtils.resexn, unit, unit, unit)
+                             MIO.dm_gmio,
+                          unit, Obj.t, unit, unit) safe_importable
+  =
+  fun fl ->
+    fun pi ->
+      fun mst ->
+        fun dcs ->
+          fun pre ->
+            fun post ->
+              fun c1post ->
+                fun c2post ->
+                  fun d1 ->
+                    fun d2 ->
+                      {
+                        ityp1 = ();
+                        c_ityp1 =
+                          (Obj.magic
+                             (Compiler_Languages.interm_arrow () () () ()
+                                (Obj.magic
+                                   (interm_exportable_super () () ()
+                                      (left dcs) d1)) ()
+                                (Obj.magic
+                                   (Compiler_Languages.interm_resexn () () ()
+                                      ()
+                                      (Obj.magic
+                                         (interm_importable_super () () ()
+                                            (right dcs) d2))))));
+                        safe_import =
+                          (fun uu___2 ->
+                             fun uu___1 ->
+                               fun uu___ ->
+                                 (fun f ->
+                                    let f = Obj.magic f in
+                                    fun eff_dcs ->
+                                      let dcs' =
+                                        EmptyNode ((left dcs), (right dcs)) in
+                                      let eff_dcs' =
+                                        EmptyNode
+                                          ((left eff_dcs), (right eff_dcs)) in
+                                      let f' =
+                                        (Obj.magic
+                                           (safe_importable_arrow () () ()
+                                              dcs' () (Obj.magic d1) ()
+                                              (Obj.magic d2))).safe_import
+                                          (Obj.magic f) eff_dcs' in
+                                      let uu___ = root eff_dcs in
+                                      match uu___ with
+                                      | Prims.Mkdtuple2 (dc_pck, eff_dc) ->
+                                          Obj.magic
+                                            (enforce_post_args_res () () ()
+                                               () ()
+                                               (rityp_idc
+                                                  (FStar_Pervasives.__proj__Mkdtuple4__item___3
+                                                     dc_pck))
+                                               (Obj.magic
+                                                  (FStar_Pervasives.__proj__Mkdtuple4__item___4
+                                                     dc_pck))
+                                               (Obj.magic
+                                                  (rityp_eff_dc () () () ()
+                                                     () ()
+                                                     (FStar_Pervasives.__proj__Mkdtuple4__item___3
+                                                        dc_pck)
+                                                     (FStar_Pervasives.__proj__Mkdtuple4__item___4
+                                                        dc_pck)
+                                                     (Obj.magic eff_dc))) ()
+                                               () f')) uu___2 uu___1 uu___)
+                      }
+let safe_importable_arrow_pre_post_res :
+  't1 't2 .
+    unit ->
+      unit ->
+        unit ->
+          unit pck_dc tree ->
+            unit ->
+              unit ->
+                unit ->
+                  unit ->
+                    ('t1, unit, Obj.t, unit, unit) exportable ->
+                      ('t2, unit, Obj.t, unit, unit) importable ->
+                        ('t1 ->
+                           ('t2 CommonUtils.resexn, unit, unit, unit)
+                             MIO.dm_gmio,
+                          unit, Obj.t, unit, unit) safe_importable
+  =
+  fun fl ->
+    fun pi ->
+      fun mst ->
+        fun dcs ->
+          fun pre ->
+            fun post ->
+              fun c1post ->
+                fun c2post ->
+                  fun d1 ->
+                    fun d2 ->
+                      {
+                        ityp1 = ();
+                        c_ityp1 =
+                          (Obj.magic
+                             (Compiler_Languages.interm_arrow () () () ()
+                                (Obj.magic
+                                   (interm_exportable_super () () ()
+                                      (left dcs) d1)) ()
+                                (Obj.magic
+                                   (Compiler_Languages.interm_resexn () () ()
+                                      ()
+                                      (Obj.magic
+                                         (interm_importable_super () () ()
+                                            (right dcs) d2))))));
+                        safe_import =
+                          (fun uu___2 ->
+                             fun uu___1 ->
+                               fun uu___ ->
+                                 (fun f ->
+                                    let f = Obj.magic f in
+                                    fun eff_dcs ->
+                                      let dcs' =
+                                        EmptyNode ((left dcs), (right dcs)) in
+                                      let eff_dcs' =
+                                        EmptyNode
+                                          ((left eff_dcs), (right eff_dcs)) in
+                                      let f' =
+                                        (Obj.magic
+                                           (safe_importable_arrow () () ()
+                                              dcs' () (Obj.magic d1) ()
+                                              (Obj.magic d2))).safe_import
+                                          (Obj.magic f) eff_dcs' in
+                                      let uu___ = root eff_dcs in
+                                      match uu___ with
+                                      | Prims.Mkdtuple2 (dc_pck, eff_dc) ->
+                                          Obj.magic
+                                            (enforce_post_res () () () () ()
+                                               (rityp_idc
+                                                  (FStar_Pervasives.__proj__Mkdtuple4__item___3
+                                                     dc_pck))
+                                               (Obj.magic
+                                                  (FStar_Pervasives.__proj__Mkdtuple4__item___4
+                                                     dc_pck))
+                                               (Obj.magic
+                                                  (rityp_eff_dc () () () ()
+                                                     () ()
+                                                     (FStar_Pervasives.__proj__Mkdtuple4__item___3
+                                                        dc_pck)
+                                                     (FStar_Pervasives.__proj__Mkdtuple4__item___4
+                                                        dc_pck)
+                                                     (Obj.magic eff_dc))) ()
+                                               () f')) uu___2 uu___1 uu___)
+                      }
+let safe_importable_arrow_pre_post_args :
+  't1 't2 .
+    unit ->
+      unit ->
+        unit ->
+          unit pck_dc tree ->
+            unit ->
+              unit ->
+                unit ->
+                  unit ->
+                    ('t1, unit, Obj.t, unit, unit) exportable ->
+                      ('t2, unit, Obj.t, unit, unit) importable ->
+                        ('t1 ->
+                           ('t2 CommonUtils.resexn, unit, unit, unit)
+                             MIO.dm_gmio,
+                          unit, Obj.t, unit, unit) safe_importable
+  =
+  fun fl ->
+    fun pi ->
+      fun mst ->
+        fun dcs ->
+          fun pre ->
+            fun post ->
+              fun c1post ->
+                fun c2post ->
+                  fun d1 ->
+                    fun d2 ->
+                      {
+                        ityp1 = ();
+                        c_ityp1 =
+                          (Obj.magic
+                             (Compiler_Languages.interm_arrow () () () ()
+                                (Obj.magic
+                                   (interm_exportable_super () () ()
+                                      (left dcs) d1)) ()
+                                (Obj.magic
+                                   (Compiler_Languages.interm_resexn () () ()
+                                      ()
+                                      (Obj.magic
+                                         (interm_importable_super () () ()
+                                            (right dcs) d2))))));
+                        safe_import =
+                          (fun uu___2 ->
+                             fun uu___1 ->
+                               fun uu___ ->
+                                 (fun f ->
+                                    let f = Obj.magic f in
+                                    fun eff_dcs ->
+                                      let dcs' =
+                                        EmptyNode ((left dcs), (right dcs)) in
+                                      let eff_dcs' =
+                                        EmptyNode
+                                          ((left eff_dcs), (right eff_dcs)) in
+                                      let f' =
+                                        (Obj.magic
+                                           (safe_importable_arrow () () ()
+                                              dcs' () (Obj.magic d1) ()
+                                              (Obj.magic d2))).safe_import
+                                          (Obj.magic f) eff_dcs' in
+                                      let uu___ = root eff_dcs in
+                                      match uu___ with
+                                      | Prims.Mkdtuple2 (dc_pck, eff_dc) ->
+                                          Obj.magic
+                                            (enforce_post_args () () () () ()
+                                               (rityp_idc
+                                                  (FStar_Pervasives.__proj__Mkdtuple4__item___3
+                                                     dc_pck))
+                                               (Obj.magic
+                                                  (FStar_Pervasives.__proj__Mkdtuple4__item___4
+                                                     dc_pck))
+                                               (Obj.magic
+                                                  (rityp_eff_dc () () () ()
+                                                     () ()
+                                                     (FStar_Pervasives.__proj__Mkdtuple4__item___3
+                                                        dc_pck)
+                                                     (FStar_Pervasives.__proj__Mkdtuple4__item___4
+                                                        dc_pck)
+                                                     (Obj.magic eff_dc))) ()
+                                               () f')) uu___2 uu___1 uu___)
+                      }
+let safe_importable_arrow_pre_post :
+  't1 't2 'pre 'post .
+    unit ->
+      unit ->
+        unit ->
+          unit pck_dc tree ->
+            unit ->
+              unit ->
+                ('t1, unit, Obj.t, unit, unit) exportable ->
+                  ('t2, unit, Obj.t, unit, unit) importable ->
+                    ('t1 ->
+                       ('t2 CommonUtils.resexn, unit, unit, unit) MIO.dm_gmio,
+                      unit, Obj.t, unit, unit) safe_importable
+  =
+  fun fl ->
+    fun pi ->
+      fun mst ->
+        fun dcs ->
+          fun c1post ->
+            fun c2post ->
+              fun d1 ->
+                fun d2 ->
+                  {
+                    ityp1 = ();
+                    c_ityp1 =
+                      (Obj.magic
+                         (Compiler_Languages.interm_arrow () () () ()
+                            (Obj.magic
+                               (interm_exportable_super () () () (left dcs)
+                                  d1)) ()
+                            (Obj.magic
+                               (Compiler_Languages.interm_resexn () () () ()
+                                  (Obj.magic
+                                     (interm_importable_super () () ()
+                                        (right dcs) d2))))));
+                    safe_import =
+                      (fun uu___2 ->
+                         fun uu___1 ->
+                           fun uu___ ->
+                             (fun f ->
+                                let f = Obj.magic f in
+                                fun eff_dcs ->
+                                  let dcs' =
+                                    EmptyNode ((left dcs), (right dcs)) in
+                                  let eff_dcs' =
+                                    EmptyNode
+                                      ((left eff_dcs), (right eff_dcs)) in
+                                  let f' =
+                                    (Obj.magic
+                                       (safe_importable_arrow () () () dcs'
+                                          () (Obj.magic d1) () (Obj.magic d2))).safe_import
+                                      (Obj.magic f) eff_dcs' in
+                                  let uu___ = root eff_dcs in
+                                  match uu___ with
+                                  | Prims.Mkdtuple2 (dc_pck, eff_dc) ->
+                                      Obj.magic
+                                        (enforce_post () () () () ()
+                                           (rityp_idc
+                                              (FStar_Pervasives.__proj__Mkdtuple4__item___3
+                                                 dc_pck))
+                                           (Obj.magic
+                                              (FStar_Pervasives.__proj__Mkdtuple4__item___4
+                                                 dc_pck))
+                                           (Obj.magic
+                                              (rityp_eff_dc () () () () () ()
+                                                 (FStar_Pervasives.__proj__Mkdtuple4__item___3
+                                                    dc_pck)
+                                                 (FStar_Pervasives.__proj__Mkdtuple4__item___4
+                                                    dc_pck)
+                                                 (Obj.magic eff_dc))) () ()
+                                           f')) uu___2 uu___1 uu___)
+                  }
