io/case-study/Execute.ml
@@ -4,14 +4,17 @@ exception Something_went_really_bad
 let (uu___is_Something_went_really_bad : Prims.exn -> Prims.bool) =
   fun projectee ->
     match projectee with | Something_went_really_bad -> true | uu___ -> false
-let rec (skip_partial_calls : Prims.int MIO_Sig.mio -> unit -> Prims.int) =
+let rec (skip_partial_calls : (unit, Prims.int) MIO_Sig.mio -> Prims.int) =
   fun tree ->
-    fun uu___ ->
-      match tree with
-      | Free.Return y -> y
-      | Free.PartialCall (pre, k) -> skip_partial_calls (k ()) ()
-      | uu___1 -> FStar_Exn.raise Something_went_really_bad
-let (execute : (unit -> (Prims.int, unit, unit) MIO.dm_gmio) -> Prims.int) =
+    match tree with
+    | Free.Return y -> y
+    | Free.PartialCall (pre, k) -> skip_partial_calls (k ())
+    | uu___ -> FStar_Exn.raise Something_went_really_bad
+let cast_mio : 'a 'wp . (unit, 'a, 'wp) MIO.dm_mio -> (unit, 'a) MIO_Sig.mio
+  = fun t -> t
+let (execute :
+  (unit -> (Prims.int, unit, unit, unit) MIO.dm_gmio) -> Prims.int) =
   fun w ->
-    let dm_tree = Obj.magic (w ()) in
-    let dm_tree' = dm_tree in skip_partial_calls dm_tree' ()
+    let dm_tree = w () in
+    let dm_tree' = dm_tree in
+    let dm_tree2 = cast_mio dm_tree' in skip_partial_calls dm_tree2
