io/Compiler.MIO.To.Interm.fst
@@ -7,6 +7,13 @@ open FStar.Ghost
 open Compiler.Languages
 open TC.Checkable
 
+let get_trace #mst () : MIOwp (Ghost.erased trace) mst GetTraceActions
+  (fun p h -> p [] (Ghost.hide h)) =
+  MIOwp?.reflect (MIO.Sig.Call.mio_call Prog GetTrace ())
+  
+let get_state #mst () : MIOwp mst.cst mst GetTraceActions
+  (fun p h -> forall s. mst.models s h ==> p [] s) =
+  MIOwp?.reflect (MIO.Sig.Call.mio_call Prog GetST ())
 
 (** **** Types **)
 (** Dynamic check possibilities:
