io/Compiler.Model1.fst
@@ -11,8 +11,16 @@ include Compiler.Languages
 include Compiler.MIO.To.Interm
 open MIO.Behavior
 
-type policy (mst:mst) (pi:policy_spec) =
-  s:mst.cst -> cmd:io_cmds -> arg:io_sig.args cmd -> r:bool{r ==> (forall h. mst.models s h ==> pi h Ctx cmd arg)}
+let static_cmd
+  (#mst:mst)
+  caller
+  (cmd : io_cmds)
+  (arg : io_sig.args cmd) :
+  MIO (io_sig.res cmd arg) mst IOActions
+    (requires (fun h -> io_pre cmd arg h))
+    (ensures (fun h (r:io_sig.res cmd arg) lt ->
+        lt == [convert_call_to_event caller cmd arg r])) =
+  MIOwp?.reflect (MIO.Sig.Call.mio_call caller cmd arg)
 
 type io_lib (fl:erased tflag) (pi:policy_spec) (mst:mst) (c:caller) =
   (cmd : io_cmds) ->
