io/Compiler.Model2.fst
@@ -11,6 +11,17 @@ include Compiler.Languages
 include Compiler.MIO.To.Interm
 open MIO.Behavior
 
+let static_cmd
+  (#mst:mst)
+  caller
+  (cmd : io_cmds)
+  (arg : io_sig.args cmd) :
+  MIO (io_sig.res cmd arg) mst IOActions
+    (requires (fun h -> io_pre cmd arg h))
+    (ensures (fun h (r:io_sig.res cmd arg) lt ->
+        lt == [convert_call_to_event caller cmd arg r])) =
+  MIOwp?.reflect (MIO.Sig.Call.mio_call caller cmd arg)
+
 type policy (pi:policy_spec) =
   h:trace -> cmd:io_cmds -> arg:io_sig.args cmd -> r:bool{r ==> pi h Ctx cmd arg}
 
