io/MIO.fst
@@ -5,7 +5,7 @@ open ExtraTactics
 open FStar.Ghost
 
 include MIO.Sig
-open MIO.Sig.Call
+//open MIO.Sig.Call
 open DMFree
 
 (** The postcondition for an io computation is defined over the
@@ -218,25 +218,9 @@ effect MIO
   (pre : trace -> Type0)
   (post : trace -> a -> trace -> Type0) =
   MIOwp a mst fl (to_hist pre post) 
-  
-let static_cmd
-  (#mst:mst)
-  caller
-  (cmd : io_cmds)
-  (arg : io_sig.args cmd) :
-  MIO (io_sig.res cmd arg) mst IOActions
-    (requires (fun h -> io_pre cmd arg h))
-    (ensures (fun h (r:io_sig.res cmd arg) lt ->
-        lt == [convert_call_to_event caller cmd arg r])) =
-  MIOwp?.reflect (mio_call caller cmd arg)
 
-let get_trace #mst () : MIOwp (Ghost.erased trace) mst GetTraceActions
-  (fun p h -> p [] (Ghost.hide h)) =
-  MIOwp?.reflect (mio_call Prog GetTrace ())
-  
-let get_state #mst () : MIOwp mst.cst mst GetTraceActions
-  (fun p h -> forall s. mst.models s h ==> p [] s) =
-  MIOwp?.reflect (mio_call Prog GetST ())
+(**
+
 
 // | GetST -> forall (x:mst.cst). mst.models x h ==> p [] x // any concrete state modelling the trace
   
