io/case-study/Monitor.fst
@@ -10,8 +10,8 @@ let monitor_state = ST.alloc my_init_cst
 
 let get_state () : St mymst.cst = !monitor_state
 
-let update_state caller (cmd:io_cmds) (argz:io_sig.args cmd) (rez:io_sig.res cmd argz) : St unit =
+let update_state (c:caller) (cmd:io_cmds) (argz:io_sig.args cmd) (rez:io_sig.res cmd argz) : St unit =
   let s0 = get_state () in
-  let e = convert_call_to_event caller cmd argz rez in
+  let e = convert_call_to_event c cmd argz rez in
   let s1 = my_update_cst s0 e in
   monitor_state := s1
